prove type_fnrec_instr and type_fn_instr

theories/typing/programs.v
@@ -12,7 +12,7 @@ Section typing.
     ∀tid vπl, lft_ctx -∗ time_ctx -∗ proph_ctx -∗ uniq_ctx -∗ elctx_interp E -∗
       na_own tid ⊤ -∗ llctx_interp L 1 -∗ cctx_interp tid C -∗ tctx_interp tid T vπl -∗
       ⟨π, pre (vπl -$ π)⟩ -∗ WP e {{ _, cont_postcondition }}.
-  Global Arguments typed_body {_} _ _ _ _ _%E _.
+  Global Arguments typed_body {_} _ _ _ _ _%E _%type.
 
   Lemma typed_body_eq {𝔄l} pre pre' E L C (T: _ 𝔄l) e :
     pre = pre' → typed_body E L C T e pre' -∗ typed_body E L C T e pre.
@@ -41,7 +41,7 @@ Section typing.
       na_own tid ⊤ -∗ llctx_interp L 1 -∗ tctx_interp tid T vπl -∗
       ⟨π, tr (postπ π) (vπl -$ π)⟩ -∗ WP e {{ v, ∃vπl', na_own tid ⊤ ∗
         llctx_interp L 1 ∗ tctx_interp tid (T' v) vπl' ∗ ⟨π, postπ π (vπl' -$ π)⟩ }}.
-  Global Arguments typed_instr {_ _} _ _ _ _%E _ _.
+  Global Arguments typed_instr {_ _} _ _ _ _%E _ _%type.
 
   (** Writing and Reading *)
 
@@ -52,7 +52,7 @@ Section typing.
       ∃(l: loc) vl, ⌜v = #l ∧ length vl = tyb.(ty_size)⌝ ∗ l ↦∗ vl ∗
         ∀wπ db, ▷ l ↦∗: tyb.(ty_own) wπ db tid -∗ ⧖(S db) ={⊤}=∗
           llctx_interp L qL ∗ ty'.(ty_own) (st ∘ vπ ⊛ wπ) (S db) tid [v].
-  Global Arguments typed_write {_ _ _} _ _ _%T _%T _%T _.
+  Global Arguments typed_write {_ _ _} _ _ _%T _%T _%T _%type.
 
   (* Technically speaking, we could remvoe the vl quantifiaction here and use
      mapsto_pred instead (i.e., l ↦∗: ty.(ty_own) tid). However, that would
@@ -65,16 +65,16 @@ Section typing.
     ty.(ty_own) vπ d tid [v] ={⊤}=∗ ∃(l: loc) vl q,
       ⌜v = #l⌝ ∗ l ↦∗{q} vl ∗ ▷ tyb.(ty_own) (gt ∘ vπ) d tid vl ∗ (l ↦∗{q} vl ={⊤}=∗
         na_own tid ⊤ ∗ llctx_interp L qL ∗ ty'.(ty_own) (st ∘ vπ) d tid [v]).
-  Global Arguments typed_read {_ _ _} _ _ _%T _%T _%T _ _.
+  Global Arguments typed_read {_ _ _} _ _ _%T _%T _%T _ _%type.
 
   Definition typed_instr_ty {𝔄l 𝔅} (E: elctx) (L: llctx)
-    (T: tctx 𝔄l) (e: expr) (ty: type 𝔅) (tr: pred 𝔅 → predl 𝔄l) : iProp Σ :=
+    (T: tctx 𝔄l) (e: expr) (ty: type 𝔅) (tr: pred' 𝔅 → predl 𝔄l) : iProp Σ :=
     typed_instr E L T e (λ v, +[v ◁ ty]) (λ post al, tr (λ b, post -[b]) al).
-  Global Arguments typed_instr_ty {_ _} _ _ _ _%E _%T _.
+  Global Arguments typed_instr_ty {_ _} _ _ _ _%E _%T _%type.
 
-  Definition typed_val {𝔄} (v: val) (ty: type 𝔄) (tr: pred (pred 𝔄)) : Prop :=
+  Definition typed_val {𝔄} (v: val) (ty: type 𝔄) (tr: pred' (pred' 𝔄)) : Prop :=
     ∀E L, ⊢ typed_instr_ty E L +[] (of_val v) ty (λ post _, tr post).
-  Global Arguments typed_val {_} _%V _%T _.
+  Global Arguments typed_val {_} _%V _%T _%type.
 
   (* This lemma is helpful when switching from proving unsafe code in Iris
      back to proving it in the type system. *)
@@ -160,7 +160,7 @@ Section typing.
   Qed.
 
   Lemma type_path_instr {𝔄} p (ty: _ 𝔄) E L :
-    ⊢ typed_instr_ty E L +[p ◁ ty] p ty (λ post '(-[v]), post v).
+    ⊢ typed_instr_ty E L +[p ◁ ty] p ty (λ post '-[v], post v).
   Proof.
     iIntros (??[vπ[]]) "_ _ _ _ _ $$ [T _] Obs". iApply (wp_hasty with "T").
     iIntros (v d _) "??". iExists -[vπ]. do 2 (iSplit; [|done]). iExists v, d.
@@ -179,7 +179,7 @@ Section typing.
   Lemma type_assign_instr {𝔄 𝔅 𝔄'} (ty: _ 𝔄) (tyb: _ 𝔅) (ty': _ 𝔄') st p pb E L :
     typed_write E L ty tyb ty' st →
     ⊢ typed_instr E L +[p ◁ ty; pb ◁ tyb] (p <- pb) (λ _, +[p ◁ ty'])
-      (λ post '(-[a; b]), post -[st a b]).
+      (λ post '-[a; b], post -[st a b]).
   Proof.
     iIntros (Wrt ?? (vπ & wπ &[])) "LFT TIME _ UNIQ E $ L (p & pb & _) Obs".
     wp_bind p. iApply (wp_hasty with "p"). iIntros (???) "_ ty".
@@ -190,7 +190,7 @@ Section typing.
     case vl=> [|?[|]]=>// ?. rewrite heap_mapsto_vec_singleton. wp_write.
     iIntros "#⧖S". iMod ("Toty'" with "[↦ tyb] ⧖S") as "($ & ty')".
     { iExists [vb]. rewrite -heap_mapsto_vec_singleton. iFrame. }
-    iExists (-[st ∘ vπ ⊛ wπ]). iFrame "Obs".
+    iExists -[st ∘ vπ ⊛ wπ]. iFrame "Obs".
     rewrite right_id tctx_hasty_val'; [|done]. iExists (S db). by iFrame.
   Qed.
 
@@ -207,7 +207,7 @@ Section typing.
   Lemma type_deref_instr {𝔄 𝔅 𝔄'} (ty: _ 𝔄) (tyb: _ 𝔅) (ty': _ 𝔄') gt st p E L :
     tyb.(ty_size) = 1 → typed_read E L ty tyb ty' gt st →
     ⊢ typed_instr E L +[p ◁ ty] (!p) (λ v, +[v ◁ tyb; p ◁ ty'])
-      (λ post '(-[a]), post -[gt a; st a]).
+      (λ post '-[a], post -[gt a; st a]).
   Proof.
     move=> Sz Read. iIntros (??[vπ[]]) "LFT _ _ _ E Na L [p _] ?".
     wp_bind p. iApply (wp_hasty with "p"). iIntros (???) "#? ty".
@@ -260,7 +260,7 @@ Section typing.
     n = tyb.(ty_size) → typed_write E L tyw tyb tyw' stw →
     typed_read E L tyr tyb tyr' gtr str →
     ⊢ typed_instr E L +[pw ◁ tyw; pr ◁ tyr] (pw <-{n} !pr)
-      (λ _, +[pw ◁ tyw'; pr ◁ tyr']) (λ post '(-[a; b]), post -[stw a (gtr b); str b]).
+      (λ _, +[pw ◁ tyw'; pr ◁ tyr']) (λ post '-[a; b], post -[stw a (gtr b); str b]).
   Proof.
     iIntros (?????(?&?&[])) "LFT TIME _ UNIQ E Na L T ?".
     iApply (type_memcpy_iris with "[$LFT $TIME $UNIQ $Na $E $L $T]")=>//. iNext.
